Example 2 almost finished; added injectivity of the KVS_serialization as a prerequisite.

aneris/examples/snapshot_isolation/examples/example2/example2_proof.v
@@ -7,6 +7,9 @@ From aneris.examples.snapshot_isolation
      Require Import snapshot_isolation_code_api.
 From iris.base_logic.lib Require Import invariants.
 From aneris.aneris_lang.lib.serialization Require Import serialization_proof.
+From aneris.examples.snapshot_isolation.instantiation
+      Require Import snapshot_isolation_api_implementation.
+Import ser_inj.
 
 Section proof_of_code.
 
@@ -18,15 +21,15 @@ Section proof_of_code.
       KVS_keys := {["x"; "y"]};
       KVS_InvName := nroot .@ "kvs_inv";
       KVS_serialization := int_serialization;
+      KVS_ser_inj := int_ser_is_ser_injective;
+      KVS_ser_inj_alt := int_ser_is_ser_injective_alt
     |}.
 
-  Context `{!anerisG Mdl Σ, !KVS_time, !KVSG Σ,
-            !KVS_snapshot_isolation_api, !SI_resources Mdl Σ}.
+  Context `{!anerisG Mdl Σ, !KVS_time, !KVSG Σ, !SI_resources Mdl Σ}.
 
   Definition local_inv_def : iProp Σ :=
-    ("x" ↦ₖ None ∗ "y" ↦ₖ None) ∨
-    (∃ w1 w2, "x" ↦ₖ Some w1 ∗ "y" ↦ₖ Some w2 ∗
-              ⌜we_val w1 = #1⌝ ∗ ⌜we_val w2 = #1⌝).
+    ∃ vx vy, "x" ↦ₖ vx ∗ "y" ↦ₖ vy ∗
+        (⌜is_Some vx⌝ -∗ ∃ w, ⌜vy = Some w⌝ ∗ ⌜we_val w = #1⌝).
 
   Definition N := nroot .@ "example".
 
@@ -46,44 +49,183 @@ Section proof_of_code.
     iIntros (Φ) "(#inv & CanStart & #start & #write & #commit) HΦ".
     rewrite/transaction1.
     wp_pures.
-    
+    wp_apply ("start" $! _ _ (⊤ ∖ ↑N)); first solve_ndisj.
+    iInv "inv" as ">(%vx & %vy & x_vx & y_vy & vx_some)" "Hclose".
+    iModIntro.
+    iExists {["x":=vx; "y":=vy]}.
+    iSplitL "CanStart x_vx y_vy"; first iFrame.
+    {
+      iApply (big_sepM_insert _ _ "x"); [done|iFrame].
+      iApply (big_sepM_insert _ _ "y"); by [|iFrame].
+    }
+    iIntros "!>(active & kv_state & snap)".
+    iPoseProof (big_sepM_insert _ _ "x" with "kv_state")
+              as "(x_vx & kv_state)"; first done.
+    iPoseProof (big_sepM_insert _ _ "y" with "kv_state")
+              as "(y_vy & _)"; first done.
+    iMod ("Hclose" with "[vx_some x_vx y_vy]").
+    { iNext. iExists vx, vy. iFrame. }
+    iModIntro.
+    wp_pures.
+    iPoseProof (big_sepM_insert _ _ "x" with "snap")
+              as "(x_vx & snap)"; first done.
+    iPoseProof (big_sepM_insert _ _ "y" with "snap")
+              as "(y_vy & _)"; first done.
+    wp_apply ("write" $! _ _ _ _ (SerVal #1) with "[] x_vx");
+            first done.
+    iIntros "x_1".
+    wp_pures.
+    wp_apply ("write" $! _ _ _ _ (SerVal #1) with "[] y_vy");
+            first done.
+    iIntros "y_1".
+    wp_pures.
+    (* TODO wait for commitT_spec to be defined *)
   Admitted.
 
   Lemma transaction2_spec cst sa :
     {{{
       local_inv ∗
-      ConnectionState cst CanStart
+      ConnectionState cst CanStart ∗
+      start_spec ∗
+      read_spec ∗
+      commit_spec
     }}}
       transaction2 cst @[ip_of_address sa]
     {{{ RET #(); True }}}.
   Proof.
+    iIntros (Φ) "(#inv & CanStart & #start & #read & #commit) HΦ".
+    rewrite/transaction2.
+    wp_pures.
+    wp_apply ("start" $! _ _ (⊤ ∖ ↑N)); first solve_ndisj.
+    iInv "inv" as ">(%vx & %vy & x_vx & y_vy & %vx_some)" "Hclose".
+    iModIntro.
+    iExists {["x":=vx; "y":=vy]}.
+    iSplitL "x_vx y_vy CanStart"; first iFrame.
+    {
+      iApply (big_sepM_insert _ _ "x"); [done|iFrame].
+      iApply (big_sepM_insert _ _ "y"); by [|iFrame].
+    }
+    iIntros "!>(active & kv_state & snap)".
+    iPoseProof (big_sepM_insert _ _ "x" with "kv_state")
+              as "(x_vx & kv_state)"; first done.
+    iPoseProof (big_sepM_insert _ _ "y" with "kv_state")
+              as "(y_vy & _)"; first done.
+    iMod ("Hclose" with "[x_vx y_vy]").
+    { iNext. iExists vx, vy. by iFrame. }
+    iModIntro.
+    wp_pures.
+    (* TODO wait for wait_on_keyT_spec to be defined *)
   Admitted.
 
   Lemma transaction1_client_spec sa :
     {{{
+      local_inv ∗
       unallocated {[sa]} ∗
       KVS_address ⤇ KVS_si ∗
       sa ⤳ (∅, ∅) ∗
-      free_ports (ip_of_address sa) {[port_of_address sa]}
+      free_ports (ip_of_address sa) {[port_of_address sa]} ∗
+      init_client_proxy_spec ∗
+      start_spec ∗
+      write_spec ∗
+      commit_spec
     }}}
       transaction1_client #sa #KVS_address @[ip_of_address sa]
     {{{ RET #(); True }}}.
   Proof.
+    iIntros (Φ) "(#inv & unalloc & #KVS_si & ∅ & free & #init & #start & #write &
+                  #commit) HΦ".
+    rewrite/transaction1_client.
+    wp_pures.
+    wp_apply ("init" with "[$unalloc $∅ $free $KVS_si]").
+    iIntros (cst) "CanStart".
+    wp_pures.
+    by wp_apply (transaction1_spec with "[$inv $start $write $commit $CanStart]").
+  Qed.
+
+  Lemma transaction2_client_spec sa :
+    {{{
+      local_inv ∗
+      unallocated {[sa]} ∗
+      KVS_address ⤇ KVS_si ∗
+      sa ⤳ (∅, ∅) ∗
+      free_ports (ip_of_address sa) {[port_of_address sa]} ∗
+      init_client_proxy_spec ∗
+      start_spec ∗
+      read_spec ∗
+      commit_spec
+    }}}
+      transaction2_client #sa #KVS_address @[ip_of_address sa]
+    {{{ RET #(); True }}}.
+  Proof.
+    iIntros (Φ) "(#inv & unalloc & #KVS_si & ∅ & free & #init & #start & #read &
+                  #commit) HΦ".
+    rewrite/transaction2_client.
+    wp_pures.
+    wp_apply ("init" with "[$unalloc $∅ $free $KVS_si]").
+    iIntros (cst) "CanStart".
+    wp_pures.
+    by wp_apply (transaction2_spec with "[$inv $start $read $commit $CanStart]").
+  Qed.
+
+End proof_of_code.
+
+(* Concrete parameters *)
+Definition addr := SocketAddressInet "0.0.0.0" 80.
+Definition clt1 := SocketAddressInet "0.0.0.1" 80.
+Definition clt2 := SocketAddressInet "0.0.0.2" 80.
+
+Definition addresses : gset socket_address := {[addr; clt1; clt2]}.
+Definition ips : gset ip_address := {["0.0.0.0"; "0.0.0.1"; "0.0.0.2"]}.
+
+Global Instance params : User_params := example2_params addr.
+
+Definition main : expr :=
+  Start "0.0.0.0" (server #KVS_address);;
+  Start "0.0.0.1" (transaction1_client #clt1 #KVS_address);;
+  Start "0.0.0.2" (transaction1_client #clt2 #KVS_address).
+
+Section proof_of_main.
+
+  Context `{!anerisG Mdl Σ, !KVS_time, !KVSG Σ, !SI_resources Mdl Σ}.
+
+  Lemma main_spec :
+    {{{
+      local_inv KVS_address ∗
+      unallocated {[clt1; clt2]} ∗
+      KVS_address ⤇ KVS_si ∗
+      KVS_address ⤳ (∅, ∅) ∗
+      clt1 ⤳ (∅, ∅) ∗
+      clt2 ⤳ (∅, ∅) ∗
+      free_ip "0.0.0.0" ∗
+      free_ip "0.0.0.1" ∗
+      free_ip "0.0.0.2" ∗
+      init_client_proxy_spec ∗
+      init_kvs_spec ∗
+      start_spec ∗
+      write_spec ∗
+      read_spec ∗
+      commit_spec ∗
+      KVS_Init
+    }}}
+      main @["system"]
+    {{{ RET #(); True }}}.
+  Proof.
+    iIntros (Φ) "(#inv & unalloc & #KVS_si & KVS_∅ & clt1_∅ & clt2_∅ &
+              free_KVS & free_clt1 & free_clt2 & #init_client & #init_kvs &
+              #start & #write & #read & #commit & KVS_Init) HΦ".
+    rewrite/main.
+    wp_apply (aneris_wp_start {[80%positive]} "0.0.0.0").
+    iSplitL "free_KVS"; first done.
+    iSplitR "KVS_∅ KVS_Init"; last first.
+    {
+      iIntros "!>free".
+      rewrite/server.
+      wp_pures.
+      by wp_apply ("init_kvs" with "[$KVS_∅ $KVS_Init $free $KVS_si]").
+    }
+    iNext.
+    wp_pures.
   Admitted.
 
 
-
-
-
-
-
-
-
-
-
-
-
-
-
-
-End proof_of_code.
+End proof_of_main.
