aneris/examples/snapshot_isolation/specs/user_params.v
@@ -1,6 +1,7 @@
 From RecordUpdate Require Import RecordSet.
 From aneris.aneris_lang Require Import network resources.
 From aneris.aneris_lang.lib.serialization Require Import serialization_proof.
+From aneris.examples.reliable_communication.prelude Require Import ser_inj.
 
 Definition Key := string.
 
@@ -11,6 +12,8 @@ Class User_params := {
   KVS_keys : gset Key;
   KVS_InvName : namespace;
   KVS_serialization : serialization;
+  KVS_ser_inj : ser_is_injective KVS_serialization;
+  KVS_ser_inj_alt : ser_is_injective_alt KVS_serialization
 }.
 
 Notation KVS_Serializable v := (Serializable KVS_serialization v).
